Tidying to Iter to make them easier to reason about
* This still needs some work and cleanup on the structure of the proofs
  etc

Valaig/Aig/Iter.lean
@@ -1,374 +1,274 @@
 module
 
-import all Valaig.Aig.Basic
-public import Valaig.Aig.ValidIn
+public import Init.Data.Iterators.Lemmas.Monadic.Basic
+public import Init.Data.Iterators.Lemmas.Basic
 
 public section
 namespace Valaig.Aig
 
-/-
-Iterator types for iterating over valid indices/variables in the Aig.
--/
-
 /--
-A generic iterator that forward iterates over a range of valid indices. This
+A generic iterator that forward iterates over a consecutive range of valid indices. This
 is specialised to produce input/latch indices and variables.
+
+This expects an instance of `Iter.Lawful` for `inc` and `valid` for full reasoning
+abilities.
 -/
-structure GenericIter {α : Type} (mk : Nat -> α) (size : Nat) (valid : α -> Prop) where
-  idx : Nat
+structure Iter {α : Type} (inc : α -> α) (valid : α -> Prop) (toNat : α -> Nat) (ofNat : Nat -> α) (size : Nat) where
+  idx : α
 
-namespace GenericIter
+namespace Iter
 
-/--
-The parameters to GenericIter are lawful if valid corresponds to the index
-being below the size. This is separated outside GenericIter to make it easier
-to infer.
--/
-class LawfulValid {α : Type} (mk : Nat -> α) (size : Nat) (valid : α -> Prop) : Prop where
-  valid : ∀ {out : α}, valid out ↔ ∃ (n : Nat) (_ : out = mk n), n < size
+class Lawful {α : Type} (inc : α -> α) (valid : α -> Prop) (toNat : α -> Nat) (ofNat : Nat -> α) (size : Nat) where
+  ofNat_toNat (idx : α) : ofNat (toNat idx) = idx := by grind
+  toNat_ofNat (idx : Nat) : toNat (ofNat idx) = idx := by grind
+  consecutive (idx : α) : toNat (inc idx) = toNat idx + 1 := by grind
+  max (idx : α) : valid idx ↔ toNat idx < size := by grind
 
-variable {α : Type} {mk : Nat -> α} {size : Nat} {valid : α -> Prop}
+variable {α : Type} {inc : α -> α} {valid : α -> Prop}
+variable {toNat : α -> Nat} {ofNat : Nat -> α} {size : Nat}
+variable [DecidablePred valid] {out : α}
 variable {m : Type -> Type _} [Pure m] {n : Type _ -> Type _}
 
-@[inline]
-instance instIterator : Std.Iterator (GenericIter mk size valid) m α where
+/--
+Construct a new iterator from the 0th index
+-/
+@[always_inline]
+def init : Iter inc valid toNat ofNat size :=
+  ⟨ofNat 0⟩
+
+@[always_inline]
+instance instIterator : Std.Iterator (Iter inc valid toNat ofNat size) m α where
   IsPlausibleStep it step :=
     let idx := it.internalState.idx
     match step with
-    | .yield it' out => idx < size ∧ it'.internalState.idx = idx + 1 ∧ out = mk idx
+    | .yield it' out => valid idx ∧ it'.internalState.idx = inc idx ∧ out = idx
     | .skip _ => False
-    | .done => idx ≥ size
+    | .done => ¬valid idx
 
   step it := pure <| .deflate <|
     let s := it.internalState
-    if h : s.idx < size then
-      .yield ⟨⟨s.idx + 1⟩⟩ (mk s.idx) (by grind)
+    if h : valid s.idx then
+      .yield ⟨⟨inc s.idx⟩⟩ s.idx (by grind)
     else
       .done (by grind)
 
-attribute [local grind =] Std.IterM.Step.toPure_yield Std.IterM.Step.toPure_skip Std.IterM.Step.toPure_done
-attribute [local grind] Std.PlausibleIterStep.yield Std.PlausibleIterStep.skip Std.PlausibleIterStep.done
-attribute [local grind =] Std.IterStep.successor_yield Std.IterStep.successor_skip Std.IterStep.successor_done
-attribute [local grind =] Std.IterStep.mapIterator_yield
-attribute [local simp, local grind] Std.Iterator.step Std.Iter.step Std.IterM.step
-attribute [local simp, local grind unfold] Std.Iter.toIterM Std.IterM.toIter
-attribute [local grind =] Std.Shrink.inflate_deflate
-attribute [local grind .] Std.Iter.IsPlausibleIndirectOutput.direct
-attribute [local grind .] Std.Iter.IsPlausibleIndirectOutput.indirect
-attribute [local simp, local grind unfold] Std.IterM.IsPlausibleStep
-attribute [local simp, local grind unfold] Std.Iter.IsPlausibleStep
-attribute [local simp, local grind unfold] Std.Iterator.IsPlausibleStep
-attribute [local simp] Std.Iter.IsPlausibleOutput
-attribute [local simp] Std.Iter.IsPlausibleSuccessorOf
-attribute [local simp, local grind unfold] Std.IterM.IsPlausibleOutput
-attribute [local simp, local grind unfold] Std.IterM.IsPlausibleSuccessorOf
+/-
+These theorems are mainly private and for establishing the correctness of the typeclasses
+-/
+variable {it it' : @Std.Iter (Iter inc valid toNat ofNat size) α}
+variable {itm itm' : @Std.IterM (Iter inc valid toNat ofNat size) m α}
+
+@[local simp, local grind =]
+private theorem IsPlausibleStep_iff {step} :
+    itm.IsPlausibleStep step ↔
+    if valid itm.internalState.idx then
+      step = .yield ⟨⟨inc itm.internalState.idx⟩⟩ itm.internalState.idx
+    else
+      step = .done := by
+  simp only [Std.IterM.IsPlausibleStep, Std.Iterator.IsPlausibleStep]
+  grind only [Iter, Std.IterM]
+
+@[local simp, local grind =]
+private theorem IsPlausibleStep_iff' {step} :
+    it.IsPlausibleStep step ↔
+    if valid it.internalState.idx then
+      step = .yield ⟨⟨inc it.internalState.idx⟩⟩ it.internalState.idx
+    else
+      step = .done := by
+  simp only [Std.Iter.IsPlausibleStep, Std.IterStep.mapIterator, Std.Iter.toIterM, Std.IterM.IsPlausibleStep, Std.Iterator.IsPlausibleStep]
+  grind only [Iter, Std.Iter]
+
+@[local simp, local grind =]
+private theorem IsPlausibleOutput_iff {out : α} :
+    itm.IsPlausibleOutput out ↔
+      valid itm.internalState.idx ∧ out = itm.internalState.idx := by
+  simp [Std.IterM.IsPlausibleOutput]
+
+omit [Pure m] in
+@[local simp, local grind =]
+private theorem successor_eq {step : Std.IterStep (@Std.IterM β m α) α} :
+    step.successor =
+    match step with
+    | .yield itm _ => some itm
+    | .skip itm => some itm
+    | .done => none := by
+  grind [Std.IterStep.successor_yield, Std.IterStep.successor_skip, Std.IterStep.successor_done]
+
+@[local simp, local grind =]
+private theorem IsPlausibleSuccessorOf_iff :
+    itm'.IsPlausibleSuccessorOf itm ↔
+      valid itm.internalState.idx ∧
+      itm'.internalState.idx = inc itm.internalState.idx := by
+  constructor
+  · grind [Std.IterM.IsPlausibleSuccessorOf]
+  · grind [Iter, Std.IterM, Std.IterM.isPlausibleSuccessorOf_of_yield (out := itm.internalState.idx)]
 
 open Std.Iterators in
-private def instFinitenessRelation : FinitenessRelation (GenericIter mk size valid) m where
-  Rel := InvImage WellFoundedRelation.rel (size - ·.internalState.idx)
+private def instFinitenessRelation [lawful : Lawful inc valid toNat ofNat size] : FinitenessRelation (Iter inc valid toNat ofNat size) m where
+  Rel := InvImage WellFoundedRelation.rel (size - toNat ·.internalState.idx)
   wf := InvImage.wf _ WellFoundedRelation.wf
-  subrelation {it it'} h := by simp_wf; grind
+  subrelation h := by simp_wf; grind [lawful.max, lawful.consecutive]
 
-instance instFinite : Std.Iterators.Finite (GenericIter mk size valid) m := by
+instance instFinite [Lawful inc valid toNat ofNat size] : Std.Iterators.Finite (Iter inc valid toNat ofNat size) m := by
   exact .of_finitenessRelation instFinitenessRelation
 
 @[always_inline]
 instance instIteratorLoop [Monad m] [Monad n] :
-    Std.IteratorLoop (GenericIter mk size valid) m n :=
+    Std.IteratorLoop (Iter inc valid toNat ofNat size) m n :=
   .defaultImplementation
 
-variable {it it' : @Std.Iter (GenericIter mk size valid) α} {out : α}
+@[local grind .]
+private theorem IsPlausibleIndirectOutput_valid {out : α} (h : itm.IsPlausibleIndirectOutput out) :
+    valid out := by
+  induction h <;> grind
 
-@[simp, grind .]
-theorem step_ne_skip {it'} :
-    it.step.val ≠ .skip it' := by
-  simp; grind
-
-@[local simp]
-private theorem successor_isSome_iff_idx_lt_size :
-    it.step.val.successor.isSome ↔ it.internalState.idx < size := by
-  simp; grind
-
-local grind_pattern successor_isSome_iff_idx_lt_size => it.step.val.successor
-
-@[local simp, local grind =]
-private theorem successor_idx_eq_idx_add_one (lt : it.internalState.idx < size) :
-    (it.step.val.successor.get (by grind) |>.internalState.idx) = it.internalState.idx + 1 := by
-  simp; grind
-
-@[local simp]
-private theorem successor_eq_idx_add_one (lt : it.internalState.idx < size) :
-    it.step.val.successor.get (by grind) = ⟨⟨it.internalState.idx + 1⟩⟩ := by
-  simp; grind
-
-local grind_pattern successor_eq_idx_add_one => it.step.val.successor
-
-@[local simp, local grind =]
-private theorem IsPlausibleOutput_iff :
-    it.IsPlausibleOutput out ↔
-      it.internalState.idx < size ∧ out = mk it.internalState.idx := by
-  simp
-  intros
-  exists ⟨⟨it.internalState.idx + 1⟩⟩
-
-@[local simp, local grind =]
-private theorem IsPlausibleSuccessorOf_iff {it' : @Std.Iter (GenericIter mk size valid) α} :
-    it'.IsPlausibleSuccessorOf it ↔
-      it.internalState.idx < size ∧
-      it'.internalState.idx = it.internalState.idx + 1 := by
-  constructor
-  · grind [Std.Iter.IsPlausibleSuccessorOf]
-  · rw [Std.Iter.isPlausibleSuccessorOf_iff_exists]
-    intros
-    exists it.step.val
-    grind [Std.Iter, GenericIter]
-
-@[local simp, local grind =]
-private theorem IsPlausibleIndirectOutput_iff :
-    it.IsPlausibleIndirectOutput out ↔
-      ∃ (n : Nat) (_ : n < size) (_ : n ≥ it.internalState.idx), mk n = out := by
-  constructor
-  · intro h
-    induction h <;> grind
-  · rintro ⟨n, h1, h2, h3⟩
-    induction h : (size - it.internalState.idx) generalizing it
-    case zero => grind
-    case succ n' ih =>
-      let it' := it.step.val.successor.get <| by grind
-      grind [Std.Iter.IsPlausibleIndirectOutput.indirect (it' := it')]
-
-@[simp, grind =]
-theorem IsPlausibleIndirectOutput_toIterM_iff :
-    it.toIterM.IsPlausibleIndirectOutput out ↔
-      ∃ (n : Nat) (_ : n < size) (_ : n ≥ it.internalState.idx), mk n = out := by
-  rw [←Std.Iter.isPlausibleIndirectOutput_iff_isPlausibleIndirectOutput_toIterM]
-  simp
-
-@[always_inline, inline]
-instance instForIn' [Monad n] [lawful : LawfulValid mk size valid] :
-    ForIn' n (@Std.Iter (GenericIter mk size valid) α) α ⟨fun _ out => valid out⟩ where
+@[always_inline]
+instance instForIn' [Monad n] :
+    ForIn' n (@Std.Iter (Iter inc valid toNat ofNat size) α) α ⟨fun _ out => valid out⟩ where
   forIn' it init f :=
     Std.IteratorLoop.finiteForIn' (fun _ _ f c => f c.run) |>.forIn' it.toIterM init
-      fun out h acc => f out (by grind [lawful.valid]) acc
-
-@[local simp, local grind =]
-private theorem length_eq_size_sub_idx :
-    it.length = size - it.internalState.idx := by
-  induction hi : size - it.internalState.idx generalizing it
-  <;> rw [Std.Iter.length_eq_match_step]
-  <;> simp
-  <;> grind
-
-@[simp]
-theorem length_lt_yield {it' out} (eq : it.step.val = .yield it' out) :
-    it'.length < it.length := by
-  grind
-
-grind_pattern length_lt_yield => it'.length < it.length, Std.IterStep.yield it' out, it.step
-grind_pattern length_lt_yield => it'.length ≤ it.length, Std.IterStep.yield it' out, it.step
-grind_pattern length_lt_yield => it'.length > it.length, Std.IterStep.yield it' out, it.step
-grind_pattern length_lt_yield => it'.length ≥ it.length, Std.IterStep.yield it' out, it.step
-
-@[simp]
-theorem length_lt_skip {it'} (eq : it.step.val = .skip it') :
-    it'.length < it.length := by
-  grind
-
-grind_pattern length_lt_skip => it'.length < it.length, Std.IterStep.skip it', it.step
-grind_pattern length_lt_skip => it'.length ≤ it.length, Std.IterStep.skip it', it.step
-grind_pattern length_lt_skip => it'.length > it.length, Std.IterStep.skip it', it.step
-grind_pattern length_lt_skip => it'.length ≥ it.length, Std.IterStep.skip it', it.step
-
-/-
-This isn't public as the ordering of elements is an implementation detail, we may wish to
-move to hashmaps or similar for inputs/latches.
--/
-@[simp, grind =]
-private theorem toList_eq_ofFn_mk_idx_add :
-    it.toList = List.ofFn (fun (n : Fin it.length) => mk (it.internalState.idx + n)) := by
-  rw [length_eq_size_sub_idx]
-  induction hi : size - it.internalState.idx generalizing it
-  · grind [Std.Iter.toList_eq_match_step]
-  · rw [Std.Iter.toList_eq_match_step]
-    split
-    · simp; grind
-    · grind
-    · simp_all; grind
-
-variable {idx : α}
-
-@[simp, grind =]
-private theorem mem_toList_iff_valid_of_idx_eq_zero [lawful : LawfulValid mk size valid]
-    (h : it.internalState.idx = 0) :
-    idx ∈ it.toList ↔ valid idx := by
-  constructor
-  · grind [@Fin.is_lt, @lawful.valid]
-  · simp
-    intro h
-    rw [lawful.valid] at h
-    rcases h with ⟨n, _⟩
-    exists ⟨n, by grind⟩
-    grind
-
-private theorem yield_idx_eq_internalState (h : it.step.val = .yield it' idx) :
-    idx = mk it.internalState.idx := by
-  grind
-
-private theorem yield_it_eq_inc (h : it.step.val = .yield it' idx) :
-    it'.internalState.idx = it.internalState.idx + 1 := by
-  grind
-
-private theorem yield_valid [lawful : LawfulValid mk size valid] (h : it.step.val = .yield it' idx) :
-    valid idx := by
-  grind [lawful.valid]
-
-private theorem done_idx_ge_size (h : it.step.val = .done) :
-    it.internalState.idx ≥ size := by
-  simp_all
-  grind
-
-end GenericIter
-
-variable {aig : Aig}
-
-section input
-
-abbrev InputIterator (aig : Aig) := GenericIter InputIdx.ofIdx aig.numInputs (·.validIn aig)
-instance {aig : Aig} : GenericIter.LawfulValid InputIdx.ofIdx aig.numInputs (·.validIn aig) where
-  valid := by grind [InputIdx.validIn, numInputs]
+      fun out h acc => f out (by grind) acc
 
 /--
-A forward iterator over inputs in the Aig.
--/
-@[inline]
-def inputs (aig : Aig) : @Std.Iter (InputIterator aig) InputIdx :=
-  ⟨⟨0⟩⟩
-
-@[simp, grind =]
-theorem length_inputs_eq_numInputs :
-    aig.inputs.length = aig.numInputs := by
-  simp [inputs, GenericIter.length_eq_size_sub_idx]
-
-@[simp, grind =]
-theorem mem_inputs_toList_iff_valid {idx : InputIdx} :
-    idx ∈ aig.inputs.toList ↔ idx.validIn aig := by
-  grind [inputs]
-
-theorem inputs_toList_ne_of_ne :
-    ∀ {i j : Nat} (hi : i < aig.numInputs) (hj : j < aig.numInputs) (_ : i ≠ j),
-      aig.inputs.toList[i]'(by simpa) ≠ aig.inputs.toList[j]'(by simpa) := by
-  simp
-
-end input
-
-section latch
-
-abbrev LatchIterator (aig : Aig) := GenericIter LatchIdx.ofIdx aig.numLatches (·.validIn aig)
-instance {aig : Aig} : GenericIter.LawfulValid LatchIdx.ofIdx aig.numLatches (·.validIn aig) where
-  valid := by grind [LatchIdx.validIn, numLatches]
-
-/--
-A forward iterator over latches in the Aig.
--/
-@[inline]
-def latches (aig : Aig) : @Std.Iter (LatchIterator aig) LatchIdx :=
-  ⟨⟨0⟩⟩
-
-@[simp, grind =]
-theorem length_latches_eq_numLatches :
-    aig.latches.length = aig.numLatches := by
-  simp [latches, GenericIter.length_eq_size_sub_idx]
-
-@[simp, grind =]
-theorem mem_latches_toList_iff_valid {idx : LatchIdx} :
-    idx ∈ aig.latches.toList ↔ idx.validIn aig := by
-  grind [latches]
-
-theorem latches_toList_ne_of_ne :
-    ∀ {i j : Nat} (hi : i < aig.numLatches) (hj : j < aig.numLatches) (_ : i ≠ j),
-      aig.latches.toList[i]'(by simpa) ≠ aig.latches.toList[j]'(by simpa) := by
-  simp
-
-end latch
-
-/-
-Forward iterators over variables
--/
-section var
-
-abbrev VarIterator (aig : Aig) := GenericIter Var.ofIdx aig.size (·.validIn aig)
-instance {aig : Aig} : GenericIter.LawfulValid Var.ofIdx aig.size (·.validIn aig) where
-  valid := by simp [Var.ext_idx, Var.validIn]
-
-/--
-A forward iterator over variables in the Aig.
--/
-@[inline]
-def iter (aig : Aig) : @Std.Iter (VarIterator aig) Var :=
-  ⟨⟨0⟩⟩
-
-@[simp, grind =]
-theorem length_iter_eq_size :
-    aig.iter.length = aig.size := by
-  simp [iter, GenericIter.length_eq_size_sub_idx]
-
-@[simp, grind =]
-theorem mem_iter_toList_iff_valid {var : Var} :
-    var ∈ aig.iter.toList ↔ var.validIn aig := by
-  grind [iter]
-
-@[simp, grind =]
-theorem iter_toList_eq :
-    aig.iter.toList = .ofFn (fun (n : Fin aig.size) => .ofIdx n) := by
-  simp
-  rw [length_iter_eq_size]
-  grind [iter]
-
-/--
-Convenience function to access the current state of `Aig.iter`, which is guaranteed to
+Convenience function to access the current state of the iterator, which is guaranteed to
 be the next returned value if the iterator is still valid.
 -/
-@[always_inline]
-def _root_.Std.Iter.var (it : @Std.Iter (VarIterator aig) Var) : Var :=
-  .ofIdx it.internalState.idx
+@[always_inline, local simp, local grind]
+def _root_.Std.Iter.val (it : @Std.Iter (Iter inc valid toNat ofNat size) α) : α :=
+  it.internalState.idx
 
-variable {it it' : @Std.Iter (VarIterator aig) Var} {var : Var}
+@[local grind =]
+theorem length_eq_size_sub_val [lawful : Lawful inc valid toNat ofNat size] :
+    it.length = size - toNat it.val := by
+  induction it using Std.Iter.inductSteps with | step it ihy _ =>
+  grind [Std.Iter.length_eq_match_step, lawful.consecutive, lawful.max]
 
-@[simp]
-theorem length_eq_size_sub_var_idx :
-    it.length = aig.size - it.var.idx := by
-  simp [Std.Iter.var, GenericIter.length_eq_size_sub_idx]
+omit [DecidablePred valid] in
+@[simp, grind! .]
+theorem val_init :
+    (⟨init⟩ : @Std.Iter (Iter inc valid toNat ofNat size) α).val = ofNat 0 := by
+  rfl
 
-@[simp, grind =]
-theorem iter_var_eq_zero :
-    aig.iter.var = .ofIdx 0 := by
-  simp [iter, Std.Iter.var]
+@[simp, grind! .]
+theorem length_init [lawful : Lawful inc valid toNat ofNat size] :
+    (⟨init⟩ : @Std.Iter (Iter inc valid toNat ofNat size) α).length = size := by
+  grind [lawful.toNat_ofNat]
 
 @[simp, grind .]
-theorem iter_yield_eq_var (h : it.step.val = .yield it' var) :
-    var = it.var := by
-  grind only [Std.Iter.var, GenericIter.yield_idx_eq_internalState]
+theorem IsPlausibleStep_skip :
+    ¬it.IsPlausibleStep (.skip it') := by
+  simp
+
+@[simp, grind .]
+theorem step_eq_iff_IsPlausibleStep {step} :
+    it.step.val = step ↔ it.IsPlausibleStep step := by
+  grind
+
+variable [lawful : Lawful inc valid toNat ofNat size]
 
 @[simp]
-theorem iter_yield_var_eq_var_add_one (h : it.step.val = .yield it' var) :
-    it'.var = it.var + 1 := by
-  simp [Std.Iter.var, Var.ext_idx]
-  grind only [GenericIter.yield_it_eq_inc]
-
-grind_pattern iter_yield_var_eq_var_add_one => Std.IterStep.yield it' var, it.var
+theorem length_yield (h : it.IsPlausibleStep (.yield it' out)) :
+    it'.length = it.length - 1 := by
+  grind [lawful.consecutive]
 
 @[simp]
-theorem iter_yield_validIn (h : it.step.val = .yield it' var) :
-    var.validIn aig := by
-  apply GenericIter.yield_valid h
-
-grind_pattern iter_yield_validIn => Std.IterStep.yield it' var, var.validIn aig, it.step
+theorem length_yield_gt_zero (h : it.IsPlausibleStep (.yield it' out)) :
+    it.length > 0 := by
+  grind [lawful.max]
 
 @[simp]
-theorem iter_done_var_ge_size (h : it.step.val = .done) :
-    it.var.idx ≥ aig.size :=
-  GenericIter.done_idx_ge_size h
+theorem length_yield' (h : it.IsPlausibleStep (.yield it' out)) :
+    it'.length + 1 = it.length := by
+  grind [length_yield, length_yield_gt_zero]
 
-grind_pattern iter_done_var_ge_size => it.step.val, Std.IterStep.done, it.var.idx
+grind_pattern length_yield' => it.IsPlausibleStep (.yield it' out), it'.length
 
-end var
+@[simp]
+theorem length_done (h : it.IsPlausibleStep .done) :
+    it.length = 0 := by
+  grind [lawful.max]
+
+grind_pattern length_done => it.IsPlausibleStep .done, it.length
+
+@[simp]
+theorem length_zero_done (h : it.length = 0) :
+    it.step.val = .done := by
+  grind [lawful.max]
+
+@[simp, grind .]
+theorem length_le_size :
+    it.length ≤ size := by
+  grind
+
+@[local grind =]
+theorem toList_eq_ofFn :
+    it.toList = List.ofFn (fun (n : Fin it.length) => ofNat (toNat it.val + n)) := by
+  induction it using Std.Iter.inductSteps with | step it ihy _ =>
+  rw [Std.Iter.toList_eq_match_step] 
+  split
+  · apply List.ext_getElem
+    · grind [lawful.consecutive, lawful.max]
+    · simp [List.getElem_cons]
+      intros
+      split
+      · simp_all only
+        grind [lawful.ofNat_toNat]
+      · grind [lawful.consecutive, lawful.max]
+  · grind
+  · grind
+
+@[simp, grind =]
+theorem toList_eq_ofFn' (h : it.val = ofNat 0) :
+    it.toList = List.ofFn (fun (n : Fin it.length) => ofNat n) := by
+  grind [lawful.toNat_ofNat]
+
+@[simp, grind =]
+theorem mem_init_toList_iff_valid {idx : α} :
+    idx ∈ (⟨init⟩ : @Std.Iter (Iter inc valid toNat ofNat size) α).toList ↔ valid idx := by
+  rw [toList_eq_ofFn']
+  simp
+  constructor
+  · grind [lawful.max, lawful.toNat_ofNat]
+  · intro valid
+    exists ⟨toNat idx, by grind [lawful.max, lawful.toNat_ofNat]⟩
+    grind [lawful.ofNat_toNat, lawful.max, lawful.toNat_ofNat]
+  · grind
+
+@[simp]
+theorem toList_done (h : it.IsPlausibleStep .done) :
+    it.toList = [] := by
+  grind
+
+grind_pattern toList_done => it.IsPlausibleStep .done, it.toList
+
+theorem toList_yield (h : it.IsPlausibleStep (.yield it' out)) :
+    it.toList = out :: it'.toList := by
+  induction h : it.toList with
+  | nil => grind [List.ofFn_eq_nil_iff, lawful.max]
+  | cons out' tail ih => grind [Std.Iter.toList_eq_match_step]
+
+grind_pattern toList_yield => it.IsPlausibleStep (.yield it' out), it.toList
+
+omit lawful in
+@[simp, grind .]
+theorem yield_eq_val (h : it.IsPlausibleStep (.yield it' out)) :
+    it.val = out := by
+  grind
+
+omit lawful in
+@[simp, grind .]
+theorem valid_yield (h : it.IsPlausibleStep (.yield it' out)) :
+    valid out := by
+  grind
+
+@[simp, grind .]
+theorem val_yield (h : it.IsPlausibleStep (.yield it' out)) :
+    toNat it'.val = toNat it.val + 1 := by
+  grind [lawful.consecutive]
+
+@[simp]
+theorem val_done (h : it.IsPlausibleStep .done) :
+    toNat it.val ≥ size := by
+  grind [lawful.max]
+
+grind_pattern val_done => it.IsPlausibleStep .done, it.val
