Valaig/Aig/Projections.lean
@@ -4,26 +4,24 @@ import all Valaig.Aig.Basic
 public import Valaig.Aig.Semantics
 public import Valaig.Aig.Iter
 
-/-
-Project out the reset and transition relation components of an Aig as new combinational Aigs.
-These may go in the future, replaced by better methods for going straight to SAT
--/
-
 public section
 namespace Valaig.Aig
 variable {aig : Aig} {wf : aig.WellFormed}
 
+/--
+Project out the reset and transition relation components of an Aig as new combinational Aigs.
+These may go in the future, replaced by better methods for going straight to SAT
+-/
 private def projectComb (aig : Aig) (reset : Bool) (wf : aig.WellFormed) : Aig × (Lit.In aig -> Lit) :=
   go aig.iter .empty (.emptyWithCapacity aig.size)
 where
   go iter (state : Aig) (map : Array Lit)
-    (size : iter.var.idx = map.size := by grind)
+    (size : iter.val.idx = map.size := by grind)
     (valid : ∀ {lit} (_ : lit ∈ map), lit.validIn state := by grind) :=
-    match h : iter.step.val with
-    | .skip it => go iter state map
-    | .done =>
+    match iter.step with
+    | .done _ =>
       ⟨state, fun lit => lit.val.mapTo <| map[lit.val.var.idx]'(by grind [Var.validIn_eq_lt_size])⟩
-    | .yield it' var =>
+    | .yield it' var _ =>
       let mapLit (lit : Lit) (h : lit.var < var := by grind) : Lit :=
         lit.mapTo map[lit.var.idx]
 
@@ -37,18 +35,16 @@ where
         | _, .and rhs0 rhs1 => state.addAnd (mapLit rhs0) (mapLit rhs1)
 
       go it' res.fst (map.push res.snd) (by simp; grind) (by simp [res]; grind)
-  termination_by iter.length
-  decreasing_by all_goals grind
+  termination_by iter.finitelyManySteps
 
 section projectComb
 variable {reset : Bool} {state : Aig} {map : Array Lit} {iter : Std.Iter Var}
-variable {size : iter.var.idx = map.size}
+variable {size : iter.val.idx = map.size}
 
 @[local simp, local grind .]
 private theorem projectComb.Comb_go (comb : state.Comb) :
     (go aig reset wf iter state map size valid).fst.Comb := by
   fun_induction go
-  · grind only
   · grind only
   next res ih =>
     apply ih
@@ -59,7 +55,6 @@ private theorem projectComb.Comb_go (comb : state.Comb) :
 private theorem projectComb.WellFormed_go (swf : state.WellFormed) :
     (go aig reset wf iter state map size valid).fst.WellFormed := by
   fun_induction go
-  · grind only
   · grind only
   next res ih =>
     apply ih
